Arithmetization/ISigmaOne/Metamath/Formula/Functions.lean
@@ -16,30 +16,30 @@ section negation
 namespace Negation
 
 def blueprint (pL : LDef) : Language.UformulaRec1.Blueprint pL where
-  rel := .mkSigma “y param n k R v | !qqNRelDef y n k R v” (by simp)
-  nrel := .mkSigma “y param n k R v | !qqRelDef y n k R v” (by simp)
-  verum := .mkSigma “y param n | !qqFalsumDef y n” (by simp)
-  falsum := .mkSigma “y param n | !qqVerumDef y n” (by simp)
-  and := .mkSigma “y param n p₁ p₂ y₁ y₂ | !qqOrDef y n y₁ y₂” (by simp)
-  or := .mkSigma “y param n p₁ p₂ y₁ y₂ | !qqAndDef y n y₁ y₂” (by simp)
-  all := .mkSigma “y param n p₁ y₁ | !qqExDef y n y₁” (by simp)
-  ex := .mkSigma “y param n p₁ y₁ | !qqAllDef y n y₁” (by simp)
-  allChanges := .mkSigma “param' param n | param' = 0” (by simp)
-  exChanges := .mkSigma “param' param n | param' = 0” (by simp)
+  rel := .mkSigma “y param k R v | !qqNRelDef y k R v” (by simp)
+  nrel := .mkSigma “y param k R v | !qqRelDef y k R v” (by simp)
+  verum := .mkSigma “y param | !qqFalsumDef y” (by simp)
+  falsum := .mkSigma “y param | !qqVerumDef y” (by simp)
+  and := .mkSigma “y param p₁ p₂ y₁ y₂ | !qqOrDef y y₁ y₂” (by simp)
+  or := .mkSigma “y param p₁ p₂ y₁ y₂ | !qqAndDef y y₁ y₂” (by simp)
+  all := .mkSigma “y param p₁ y₁ | !qqExDef y y₁” (by simp)
+  ex := .mkSigma “y param p₁ y₁ | !qqAllDef y y₁” (by simp)
+  allChanges := .mkSigma “param' param | param' = 0” (by simp)
+  exChanges := .mkSigma “param' param | param' = 0” (by simp)
 
 variable (L)
 
 def construction : Language.UformulaRec1.Construction V L (blueprint pL) where
-  rel {_} := fun n k R v ↦ ^nrel n k R v
-  nrel {_} := fun n k R v ↦ ^rel n k R v
-  verum {_} := fun n ↦ ^⊥[n]
-  falsum {_} := fun n ↦ ^⊤[n]
-  and {_} := fun n _ _ y₁ y₂ ↦ y₁ ^⋎[n] y₂
-  or {_} := fun n _ _ y₁ y₂ ↦ y₁ ^⋏[n] y₂
-  all {_} := fun n _ y₁ ↦ ^∃[n] y₁
-  ex {_} := fun n _ y₁ ↦ ^∀[n] y₁
-  allChanges := fun _ _ ↦ 0
-  exChanges := fun _ _ ↦ 0
+  rel {_} := fun k R v ↦ ^nrel k R v
+  nrel {_} := fun k R v ↦ ^rel k R v
+  verum {_} := ^⊥
+  falsum {_} := ^⊤
+  and {_} := fun _ _ y₁ y₂ ↦ y₁ ^⋎ y₂
+  or {_} := fun _ _ y₁ y₂ ↦ y₁ ^⋏ y₂
+  all {_} := fun _ y₁ ↦ ^∃ y₁
+  ex {_} := fun _ y₁ ↦ ^∀ y₁
+  allChanges := fun _ ↦ 0
+  exChanges := fun _ ↦ 0
   rel_defined := by intro v; simp [blueprint]; rfl
   nrel_defined := by intro v; simp [blueprint]; rfl
   verum_defined := by intro v; simp [blueprint]
@@ -67,124 +67,134 @@ def _root_.LO.FirstOrder.Arith.LDef.negDef (pL : LDef) : 𝚺₁.Semisentence 2 
 
 variable (L)
 
-lemma neg_defined : 𝚺₁-Function₁ L.neg via pL.negDef := fun v ↦ by
+lemma Language.neg_defined : 𝚺₁-Function₁ L.neg via pL.negDef := fun v ↦ by
   simpa [LDef.negDef] using (construction L).result_defined ![v 0, 0, v 1]
 
-@[simp] lemma neg_defined_iff (v : Fin 2 → V) :
-    Semiformula.Evalbm (L := ℒₒᵣ) V v pL.negDef ↔ v 0 = L.neg (v 1) := (neg_defined L).df.iff v
+instance Language.neg_definable : 𝚺₁-Function₁ L.neg := L.neg_defined.to_definable
 
-instance neg_definable : 𝚺₁-Function₁ L.neg :=
-  (neg_defined L).to_definable
-
-instance neg_definable' (Γ) : Γ-[m + 1]-Function₁ L.neg :=
-  .of_sigmaOne (neg_definable L) _ _
+instance Language.neg_definable' (Γ) : Γ-[m + 1]-Function₁ L.neg :=
+  .of_sigmaOne (neg_definable L)
 
 end
 
-@[simp] lemma neg_rel {n k R v} (hR : L.Rel k R) (hv : L.SemitermVec k n v) :
-    L.neg (^rel n k R v) = ^nrel n k R v := by simp [Language.neg, hR, hv, construction]
+@[simp] lemma neg_rel {k R v} (hR : L.Rel k R) (hv : L.IsUTermVec k v) :
+    L.neg (^rel k R v) = ^nrel k R v := by simp [Language.neg, hR, hv, construction]
 
-@[simp] lemma neg_nrel {n k R v} (hR : L.Rel k R) (hv : L.SemitermVec k n v) :
-    L.neg (^nrel n k R v) = ^rel n k R v := by simp [Language.neg, hR, hv, construction]
+@[simp] lemma neg_nrel {k R v} (hR : L.Rel k R) (hv : L.IsUTermVec k v) :
+    L.neg (^nrel k R v) = ^rel k R v := by simp [Language.neg, hR, hv, construction]
 
-@[simp] lemma neg_verum (n) :
-    L.neg ^⊤[n] = ^⊥[n] := by simp [Language.neg, construction]
+@[simp] lemma neg_verum :
+    L.neg ^⊤ = ^⊥ := by simp [Language.neg, construction]
 
-@[simp] lemma neg_falsum (n) :
-    L.neg ^⊥[n] = ^⊤[n] := by simp [Language.neg, construction]
+@[simp] lemma neg_falsum :
+    L.neg ^⊥ = ^⊤ := by simp [Language.neg, construction]
 
-@[simp] lemma neg_and {n p q} (hp : L.Semiformula n p) (hq : L.Semiformula n q) :
-    L.neg (p ^⋏[n] q) = L.neg p ^⋎[n] L.neg q := by simp [Language.neg, hp, hq, construction]
+@[simp] lemma neg_and {p q} (hp : L.IsUFormula p) (hq : L.IsUFormula q) :
+    L.neg (p ^⋏ q) = L.neg p ^⋎ L.neg q := by simp [Language.neg, hp, hq, construction]
 
-@[simp] lemma neg_or {n p q} (hp : L.Semiformula n p) (hq : L.Semiformula n q) :
-    L.neg (p ^⋎[n] q) = L.neg p ^⋏[n] L.neg q := by simp [Language.neg, hp, hq, construction]
+@[simp] lemma neg_or {p q} (hp : L.IsUFormula p) (hq : L.IsUFormula q) :
+    L.neg (p ^⋎ q) = L.neg p ^⋏ L.neg q := by simp [Language.neg, hp, hq, construction]
 
-@[simp] lemma neg_all {n p} (hp : L.Semiformula (n + 1) p) :
-    L.neg (^∀[n] p) = ^∃[n] (L.neg p) := by simp [Language.neg, hp, construction]
+@[simp] lemma neg_all {p} (hp : L.IsUFormula p) :
+    L.neg (^∀ p) = ^∃ (L.neg p) := by simp [Language.neg, hp, construction]
 
-@[simp] lemma neg_ex {n p} (hp : L.Semiformula (n + 1) p) :
-    L.neg (^∃[n] p) = ^∀[n] (L.neg p) := by simp [Language.neg, hp, construction]
+@[simp] lemma neg_ex {p} (hp : L.IsUFormula p) :
+    L.neg (^∃ p) = ^∀ (L.neg p) := by simp [Language.neg, hp, construction]
 
-lemma neg_not_uformula {x} (h : ¬L.UFormula x) :
+lemma neg_not_uformula {x} (h : ¬L.IsUFormula x) :
     L.neg x = 0 := (construction L).result_prop_not _ h
 
-lemma fstIdx_neg {p} (h : L.UFormula p) : fstIdx (L.neg p) = fstIdx p := by
-  rcases h.case with (⟨_, _, _, _, _, _, rfl⟩ | ⟨_, _, _, _, _, _, rfl⟩ | ⟨_, rfl⟩ | ⟨_, rfl⟩ |
-    ⟨_, _, _, _, _, rfl⟩ | ⟨_, _, _, _, _, rfl⟩ | ⟨_, _, _, rfl⟩ | ⟨_, _, _, rfl⟩) <;>
-    simp [*]
-
-lemma Language.Semiformula.neg {p : V} : L.Semiformula n p → L.Semiformula n (L.neg p) := by
-  apply Language.Semiformula.induction_sigma₁
+lemma Language.IsUFormula.neg {p : V} : L.IsUFormula p → L.IsUFormula (L.neg p) := by
+  apply Language.IsUFormula.induction_sigma1
   · definability
-  · intro n k r v hr hv; simp [hr, hv]
-  · intro n k r v hr hv; simp [hr, hv]
+  · intro k r v hr hv; simp [hr, hv]
+  · intro k r v hr hv; simp [hr, hv]
   · simp
   · simp
-  · intro n p q hp hq ihp ihq; simp [hp, hq, ihp, ihq]
-  · intro n p q hp hq ihp ihq; simp [hp, hq, ihp, ihq]
-  · intro n p hp ihp; simp [hp, ihp]
-  · intro n p hp ihp; simp [hp, ihp]
+  · intro p q hp hq ihp ihq; simp [hp, hq, ihp, ihq]
+  · intro p q hp hq ihp ihq; simp [hp, hq, ihp, ihq]
+  · intro p hp ihp; simp [hp, ihp]
+  · intro p hp ihp; simp [hp, ihp]
 
-@[simp] lemma Language.Semiformula.neg_iff {p : V} : L.Semiformula n (L.neg p) ↔ L.Semiformula n p :=
-  ⟨fun h ↦ by
-    rcases h with ⟨h, rfl⟩
-    have : L.UFormula p := by
-      by_contra hp
-      simp [neg_not_uformula hp] at h
-    exact ⟨this, by simp [fstIdx_neg this]⟩,
-    Language.Semiformula.neg⟩
-
-@[simp] lemma neg_neg {p : V} : L.Semiformula n p → L.neg (L.neg p) = p := by
-  apply Language.Semiformula.induction_sigma₁
+@[simp] lemma Language.IsUFormula.bv_neg {p : V} : L.IsUFormula p → L.bv (L.neg p) = L.bv p := by
+  apply Language.IsUFormula.induction_sigma1
   · definability
-  · intro n k r v hr hv; simp [hr, hv]
-  · intro n k r v hr hv; simp [hr, hv]
-  · intro n; simp
-  · intro n; simp
-  · intro n p q hp hq ihp ihq; simp [hp, hq, ihp, ihq]
-  · intro n p q hp hq ihp ihq; simp [hp, hq, ihp, ihq]
-  · intro n p hp ihp; simp [hp, ihp]
-  · intro n p hp ihp; simp [hp, ihp]
+  · intro k R v hR hv; simp [*]
+  · intro k R v hR hv; simp [*]
+  · simp
+  · simp
+  · intro p q hp hq ihp ihq; simp [hp, hq, hp.neg, hq.neg, ihp, ihq]
+  · intro p q hp hq ihp ihq; simp [hp, hq, hp.neg, hq.neg, ihp, ihq]
+  · intro p hp ihp; simp [hp, hp.neg, ihp]
+  · intro p hp ihp; simp [hp, hp.neg, ihp]
 
-@[simp] lemma neg_inj_iff (hp : L.Semiformula n p) (hq : L.Semiformula n q) : L.neg p = L.neg q ↔ p = q := by
+@[simp] lemma Language.IsUFormula.neg_neg {p : V} : L.IsUFormula p → L.neg (L.neg p) = p := by
+  apply Language.IsUFormula.induction_sigma1
+  · definability
+  · intro k r v hr hv; simp [hr, hv]
+  · intro k r v hr hv; simp [hr, hv]
+  · simp
+  · simp
+  · intro p q hp hq ihp ihq; simp [hp, hq, hp.neg, hq.neg, ihp, ihq]
+  · intro p q hp hq ihp ihq; simp [hp, hq, hp.neg, hq.neg, ihp, ihq]
+  · intro p hp ihp; simp [hp, hp.neg, ihp]
+  · intro p hp ihp; simp [hp, hp.neg, ihp]
+
+@[simp] lemma Language.IsUFormula.neg_iff {p : V} : L.IsUFormula (L.neg p) ↔ L.IsUFormula p := by
   constructor
-  · intro h; simpa [neg_neg hp, neg_neg hq] using congrArg L.neg h
+  · intro h; by_contra hp
+    have Hp : L.IsUFormula p := by by_contra hp; simp [neg_not_uformula hp] at h
+    contradiction
+  · exact Language.IsUFormula.neg
+
+@[simp] lemma Language.IsSemiformula.neg_iff {p : V} : L.IsSemiformula n (L.neg p) ↔ L.IsSemiformula n p := by
+  constructor
+  · intro h; by_contra hp
+    have Hp : L.IsUFormula p := by by_contra hp; simp [neg_not_uformula hp] at h
+    have : L.IsSemiformula n p := ⟨Hp, by simpa [Hp.bv_neg] using h.bv⟩
+    contradiction
+  · intro h; exact ⟨by simp [h.isUFormula], by simpa [h.isUFormula] using h.bv⟩
+
+alias ⟨Language.IsSemiformula.elim_neg, Language.IsSemiformula.neg⟩ := Language.IsSemiformula.neg_iff
+
+@[simp] lemma neg_inj_iff (hp : L.IsUFormula p) (hq : L.IsUFormula q) : L.neg p = L.neg q ↔ p = q := by
+  constructor
+  · intro h; simpa [hp.neg_neg, hq.neg_neg] using congrArg L.neg h
   · rintro rfl; rfl
 
 end negation
 
 variable (L)
 
-def Language.imp (n p q : V) : V := L.neg p ^⋎[n] q
+def Language.imp (p q : V) : V := L.neg p ^⋎ q
 
-notation:60 p:61 " ^→[" L "; " n "] " q:60 => Language.imp L n p q
+notation:60 p:61 " ^→[" L "] " q:60 => Language.imp L p q
 
 variable {L}
 
 section imp
 
-@[simp] lemma Language.Semiformula.imp {n p q : V} :
-    L.Semiformula n (L.imp n p q) ↔ L.Semiformula n p ∧ L.Semiformula n q := by
+@[simp] lemma Language.IsUFormula.imp {p q : V} :
+    L.IsUFormula (L.imp p q) ↔ L.IsUFormula p ∧ L.IsUFormula q := by
+  simp [Language.imp]
+
+@[simp] lemma Language.IsSemiformula.imp {n p q : V} :
+    L.IsSemiformula n (L.imp p q) ↔ L.IsSemiformula n p ∧ L.IsSemiformula n q := by
   simp [Language.imp]
 
 section
 
-def _root_.LO.FirstOrder.Arith.LDef.impDef (pL : LDef) : 𝚺₁.Semisentence 4 := .mkSigma
-  “r n p q | ∃ np, !pL.negDef np p ∧ !qqOrDef r n np q” (by simp)
+def _root_.LO.FirstOrder.Arith.LDef.impDef (pL : LDef) : 𝚺₁.Semisentence 3 := .mkSigma
+  “r p q | ∃ np, !pL.negDef np p ∧ !qqOrDef r np q” (by simp)
 
 variable (L)
 
-lemma imp_defined : 𝚺₁-Function₃ L.imp via pL.impDef := fun v ↦ by
-  simp [LDef.impDef, (neg_defined L).df.iff]; rfl
+lemma Language.imp_defined : 𝚺₁-Function₂ L.imp via pL.impDef := fun v ↦ by
+  simp [LDef.impDef, L.neg_defined.df.iff]; rfl
 
-@[simp] lemma eval_impDef (v : Fin 4 → V) :
-    Semiformula.Evalbm V v pL.impDef.val ↔ v 0 = L.imp (v 1) (v 2) (v 3) := (imp_defined L).df.iff v
+instance Language.imp_definable : 𝚺₁-Function₂ L.imp := L.imp_defined.to_definable
 
-instance imp_definable : 𝚺₁-Function₃ L.imp :=
-  (imp_defined L).to_definable
-
-instance imp_definable' (Γ) : Γ-[m + 1]-Function₃ L.imp :=
-  .of_sigmaOne (imp_definable L) _ _
+instance imp_definable' : Γ-[m + 1]-Function₂ L.imp := L.imp_definable.of_sigmaOne
 
 end
 
@@ -195,32 +205,32 @@ section shift
 namespace Shift
 
 def blueprint (pL : LDef) : Language.UformulaRec1.Blueprint pL where
-  rel := .mkSigma “y param n k R v | ∃ v', !pL.termShiftVecDef v' k n v ∧ !qqRelDef y n k R v'” (by simp)
-  nrel := .mkSigma “y param n k R v | ∃ v', !pL.termShiftVecDef v' k n v ∧ !qqNRelDef y n k R v'” (by simp)
-  verum := .mkSigma “y param n | !qqVerumDef y n” (by simp)
-  falsum := .mkSigma “y param n | !qqFalsumDef y n” (by simp)
-  and := .mkSigma “y param n p₁ p₂ y₁ y₂ | !qqAndDef y n y₁ y₂” (by simp)
-  or := .mkSigma “y param n p₁ p₂ y₁ y₂ | !qqOrDef y n y₁ y₂” (by simp)
-  all := .mkSigma “y param n p₁ y₁ | !qqAllDef y n y₁” (by simp)
-  ex := .mkSigma “y param n p₁ y₁ | !qqExDef y n y₁” (by simp)
-  allChanges := .mkSigma “param' param n | param' = 0” (by simp)
-  exChanges := .mkSigma “param' param n | param' = 0” (by simp)
+  rel := .mkSigma “y param k R v | ∃ v', !pL.termShiftVecDef v' k v ∧ !qqRelDef y k R v'” (by simp)
+  nrel := .mkSigma “y param k R v | ∃ v', !pL.termShiftVecDef v' k v ∧ !qqNRelDef y k R v'” (by simp)
+  verum := .mkSigma “y param | !qqVerumDef y” (by simp)
+  falsum := .mkSigma “y param | !qqFalsumDef y” (by simp)
+  and := .mkSigma “y param p₁ p₂ y₁ y₂ | !qqAndDef y y₁ y₂” (by simp)
+  or := .mkSigma “y param p₁ p₂ y₁ y₂ | !qqOrDef y y₁ y₂” (by simp)
+  all := .mkSigma “y param p₁ y₁ | !qqAllDef y y₁” (by simp)
+  ex := .mkSigma “y param p₁ y₁ | !qqExDef y y₁” (by simp)
+  allChanges := .mkSigma “param' param | param' = 0” (by simp)
+  exChanges := .mkSigma “param' param | param' = 0” (by simp)
 
 variable (L)
 
 def construction : Language.UformulaRec1.Construction V L (blueprint pL) where
-  rel {_} := fun n k R v ↦ ^rel n k R (L.termShiftVec k n v)
-  nrel {_} := fun n k R v ↦ ^nrel n k R (L.termShiftVec k n v)
-  verum {_} := fun n ↦ ^⊤[n]
-  falsum {_} := fun n ↦ ^⊥[n]
-  and {_} := fun n _ _ y₁ y₂ ↦ y₁ ^⋏[n] y₂
-  or {_} := fun n _ _ y₁ y₂ ↦ y₁ ^⋎[n] y₂
-  all {_} := fun n _ y₁ ↦ ^∀[n] y₁
-  ex {_} := fun n _ y₁ ↦ ^∃[n] y₁
-  allChanges := fun _ _ ↦ 0
-  exChanges := fun _ _ ↦ 0
-  rel_defined := by intro v; simp [blueprint, (termShiftVec_defined L).df.iff]; rfl
-  nrel_defined := by intro v; simp [blueprint, (termShiftVec_defined L).df.iff]; rfl
+  rel {_} := fun k R v ↦ ^rel k R (L.termShiftVec k v)
+  nrel {_} := fun k R v ↦ ^nrel k R (L.termShiftVec k v)
+  verum {_} := ^⊤
+  falsum {_} := ^⊥
+  and {_} := fun _ _ y₁ y₂ ↦ y₁ ^⋏ y₂
+  or {_} := fun _ _ y₁ y₂ ↦ y₁ ^⋎ y₂
+  all {_} := fun _ y₁ ↦ ^∀ y₁
+  ex {_} := fun _ y₁ ↦ ^∃ y₁
+  allChanges := fun _ ↦ 0
+  exChanges := fun _ ↦ 0
+  rel_defined := by intro v; simp [blueprint, L.termShiftVec_defined.df.iff]; rfl
+  nrel_defined := by intro v; simp [blueprint, L.termShiftVec_defined.df.iff]; rfl
   verum_defined := by intro v; simp [blueprint]
   falsum_defined := by intro v; simp [blueprint]
   and_defined := by intro v; simp [blueprint]; rfl
@@ -246,84 +256,75 @@ def _root_.LO.FirstOrder.Arith.LDef.shiftDef (pL : LDef) : 𝚺₁.Semisentence 
 
 variable (L)
 
-lemma shift_defined : 𝚺₁-Function₁ L.shift via pL.shiftDef := fun v ↦ by
+lemma Language.shift_defined : 𝚺₁-Function₁ L.shift via pL.shiftDef := fun v ↦ by
   simpa [LDef.shiftDef] using (construction L).result_defined ![v 0, 0, v 1]
 
-@[simp] lemma eval_shiftDef (v : Fin 2 → V) :
-    Semiformula.Evalbm (L := ℒₒᵣ) V v pL.shiftDef ↔ v 0 = L.shift (v 1) := (shift_defined L).df.iff v
+instance Language.shift_definable : 𝚺₁-Function₁ L.shift := L.shift_defined.to_definable
 
-instance shift_definable : 𝚺₁-Function₁ L.shift :=
-  (shift_defined L).to_definable
-
-instance shift_definable' (Γ) : Γ-[m + 1]-Function₁ L.shift :=
-  .of_sigmaOne (shift_definable L) _ _
+instance language.shift_definable' : Γ-[m + 1]-Function₁ L.shift := L.shift_definable.of_sigmaOne
 
 end
 
-@[simp] lemma shift_rel {n k R v} (hR : L.Rel k R) (hv : L.SemitermVec k n v) :
-    L.shift (^rel n k R v) = ^rel n k R (L.termShiftVec k n v) := by simp [Language.shift, hR, hv, construction]
+@[simp] lemma shift_rel {k R v} (hR : L.Rel k R) (hv : L.IsUTermVec k v) :
+    L.shift (^relk R v) = ^relk R (L.termShiftVec k v) := by simp [Language.shift, hR, hv, construction]
 
-@[simp] lemma shift_nrel {n k R v} (hR : L.Rel k R) (hv : L.SemitermVec k n v) :
-    L.shift (^nrel n k R v) = ^nrel n k R (L.termShiftVec k n v) := by simp [Language.shift, hR, hv, construction]
+@[simp] lemma shift_nrel {k R v} (hR : L.Rel k R) (hv : L.IsUTermVec k v) :
+    L.shift (^nrelk R v) = ^nrelk R (L.termShiftVec k v) := by simp [Language.shift, hR, hv, construction]
 
-@[simp] lemma shift_verum (n) :
-    L.shift ^⊤[n] = ^⊤[n] := by simp [Language.shift, construction]
+@[simp] lemma shift_verum : L.shift ^⊤ = ^⊤ := by simp [Language.shift, construction]
 
-@[simp] lemma shift_falsum (n) :
-    L.shift ^⊥[n] = ^⊥[n] := by simp [Language.shift, construction]
+@[simp] lemma shift_falsum : L.shift ^⊥ = ^⊥ := by simp [Language.shift, construction]
 
-@[simp] lemma shift_and {n p q} (hp : L.Semiformula n p) (hq : L.Semiformula n q) :
-    L.shift (p ^⋏[n] q) = L.shift p ^⋏[n] L.shift q := by simp [Language.shift, hp, hq, construction]
+@[simp] lemma shift_and {p q} (hp : L.IsUFormula p) (hq : L.IsUFormula q) :
+    L.shift (p ^⋏ q) = L.shift p ^⋏ L.shift q := by simp [Language.shift, hp, hq, construction]
 
-@[simp] lemma shift_or {n p q} (hp : L.Semiformula n p) (hq : L.Semiformula n q) :
-    L.shift (p ^⋎[n] q) = L.shift p ^⋎[n] L.shift q := by simp [Language.shift, hp, hq, construction]
+@[simp] lemma shift_or {p q} (hp : L.IsUFormula p) (hq : L.IsUFormula q) :
+    L.shift (p ^⋎ q) = L.shift p ^⋎ L.shift q := by simp [Language.shift, hp, hq, construction]
 
-@[simp] lemma shift_all {n p} (hp : L.Semiformula (n + 1) p) :
-    L.shift (^∀[n] p) = ^∀[n] (L.shift p) := by simp [Language.shift, hp, construction]
+@[simp] lemma shift_all {p} (hp : L.IsUFormula p) :
+    L.shift (^∀ p) = ^∀ (L.shift p) := by simp [Language.shift, hp, construction]
 
-@[simp] lemma shift_ex {n p} (hp : L.Semiformula (n + 1) p) :
-    L.shift (^∃[n] p) = ^∃[n] (L.shift p) := by simp [Language.shift, hp, construction]
+@[simp] lemma shift_ex {p} (hp : L.IsUFormula p) :
+    L.shift (^∃ p) = ^∃ (L.shift p) := by simp [Language.shift, hp, construction]
 
-lemma shift_not_uformula {x} (h : ¬L.UFormula x) :
+lemma shift_not_uformula {x} (h : ¬L.IsUFormula x) :
     L.shift x = 0 := (construction L).result_prop_not _ h
 
-lemma Language.Semiformula.shift {p : V} : L.Semiformula n p → L.Semiformula n (L.shift p) := by
-  apply Language.Semiformula.induction_sigma₁
+lemma Language.IsSemiformula.shift {p : V} : L.IsSemiformula n p → L.IsSemiformula n (L.shift p) := by
+  apply Language.IsSemiformula.induction_sigma1
   · definability
-  · intro n k r v hr hv; simp [hr, hv]
-  · intro n k r v hr hv; simp [hr, hv]
+  · intro n k r v hr hv; simp [hr, hv, hv.isUTerm]
+  · intro n k r v hr hv; simp [hr, hv, hv.isUTerm]
   · simp
   · simp
-  · intro n p q hp hq ihp ihq; simp [hp, hq, ihp, ihq]
-  · intro n p q hp hq ihp ihq; simp [hp, hq, ihp, ihq]
-  · intro n p hp ihp; simp [hp, ihp]
-  · intro n p hp ihp; simp [hp, ihp]
+  · intro n p q hp hq ihp ihq; simp [hp, hq, hp.isUFormula, hq.isUFormula, ihp, ihq]
+  · intro n p q hp hq ihp ihq; simp [hp, hq, hp.isUFormula, hq.isUFormula, ihp, ihq]
+  · intro n p hp ihp; simp [hp, hp.isUFormula, ihp]
+  · intro n p hp ihp; simp [hp, hp.isUFormula, ihp]
 
-lemma fstIdx_shift {p} (h : L.UFormula p) : fstIdx (L.shift p) = fstIdx p := by
-  rcases h.case with (⟨_, _, _, _, _, _, rfl⟩ | ⟨_, _, _, _, _, _, rfl⟩ | ⟨_, rfl⟩ | ⟨_, rfl⟩ |
-    ⟨_, _, _, _, _, rfl⟩ | ⟨_, _, _, _, _, rfl⟩ | ⟨_, _, _, rfl⟩ | ⟨_, _, _, rfl⟩) <;>
-    simp [*]
-
-@[simp] lemma Language.Semiformula.shift_iff {p : V} : L.Semiformula n (L.shift p) ↔ L.Semiformula n p :=
+/-
+@[simp] lemma Language.IsSemiformula.shift_iff {p : V} : L.Semiformula n (L.shift p) ↔ L.Semiformula n p :=
   ⟨fun h ↦ by
     rcases h with ⟨h, rfl⟩
     have : L.UFormula p := by
       by_contra hp
       simp [shift_not_uformula hp] at h
     exact ⟨this, by simp [fstIdx_shift this]⟩,
-    Language.Semiformula.shift⟩
+    Language.IsSemiformula.shift⟩
+-/
 
-lemma shift_neg {p : V} (hp : L.Semiformula n p) : L.shift (L.neg p) = L.neg (L.shift p) := by
-  apply Language.Semiformula.induction_sigma₁ ?_ ?_ ?_ ?_ ?_ ?_ ?_ ?_ ?_ _ _ hp
+
+lemma shift_neg {p : V} (hp : L.IsSemiformula n p) : L.shift (L.neg p) = L.neg (L.shift p) := by
+  apply Language.IsSemiformula.induction_sigma1 ?_ ?_ ?_ ?_ ?_ ?_ ?_ ?_ ?_ hp
   · definability
-  · intro n k R v hR hv; simp [*]
-  · intro n k R v hR hv; simp [*]
-  · intro n; simp
-  · intro n; simp
-  · intro n p q hp hq ihp ihq; simp [*]
-  · intro n p q hp hq ihp ihq; simp [*]
-  · intro n p hp ih; simp [*]
-  · intro n p hp ih; simp [*]
+  · intro n k R v hR hv; simp [hR, hv.isUTerm, hv.termShiftVec.isUTerm]
+  · intro n k R v hR hv; simp [hR, hv.isUTerm, hv.termShiftVec.isUTerm]
+  · simp
+  · simp
+  · intro n p q hp hq ihp ihq; simp [hp.isUFormula, hq.isUFormula, hp.shift.isUFormula, hq.shift.isUFormula, ihp, ihq]
+  · intro n p q hp hq ihp ihq; simp [hp.isUFormula, hq.isUFormula, hp.shift.isUFormula, hq.shift.isUFormula, ihp, ihq]
+  · intro n p hp ih; simp [hp.isUFormula, hp.shift.isUFormula, ih]
+  · intro n p hp ih; simp [hp.isUFormula, hp.shift.isUFormula, ih]
 
 end shift
 
@@ -333,55 +334,55 @@ section
 
 variable (L)
 
-def _root_.LO.FirstOrder.Arith.LDef.qVecDef (pL : LDef) : 𝚺₁.Semisentence 4 := .mkSigma
-  “w' k n w | ∃ sw, !pL.termBShiftVecDef sw k n w ∧ ∃ t, !qqBvarDef t 0 ∧ !consDef w' t sw” (by simp)
+def _root_.LO.FirstOrder.Arith.LDef.qVecDef (pL : LDef) : 𝚺₁.Semisentence 2 := .mkSigma
+  “w' w | ∃ k, !lenDef k w ∧ ∃ sw, !pL.termBShiftVecDef sw k w ∧ ∃ t, !qqBvarDef t 0 ∧ !consDef w' t sw” (by simp)
 
-lemma qVec_defined : 𝚺₁-Function₃ L.qVec via pL.qVecDef := by
-  intro v; simp [LDef.qVecDef, eval_termBShiftVecDef L]; rfl
+lemma Language.qVec_defined : 𝚺₁-Function₁ L.qVec via pL.qVecDef := by
+  intro v; simp [LDef.qVecDef, L.termBShiftVec_defined.df.iff]; rfl
 
-instance qVec_definable : 𝚺₁-Function₃ L.qVec := (qVec_defined L).to_definable
+instance Language.qVec_definable : 𝚺₁-Function₁ L.qVec := L.qVec_defined.to_definable
 
-@[simp, definability] instance qVec_definable' (Γ m) : Γ-[m + 1]-Function₃ L.qVec := .of_sigmaOne (qVec_definable L) _ _
+instance Language.qVec_definable' : Γ-[m + 1]-Function₁ L.qVec := L.qVec_definable.of_sigmaOne
 
 end
 
 namespace Substs
 
 def blueprint (pL : LDef) : Language.UformulaRec1.Blueprint pL where
-  rel    := .mkSigma “y param n k R v | ∃ m, !pi₁Def m param ∧ ∃ w, !pi₂Def w param ∧ ∃ v', !pL.termSubstVecDef v' k n m w v ∧ !qqRelDef y m k R v'” (by simp)
-  nrel   := .mkSigma “y param n k R v | ∃ m, !pi₁Def m param ∧ ∃ w, !pi₂Def w param ∧ ∃ v', !pL.termSubstVecDef v' k n m w v ∧ !qqNRelDef y m k R v'” (by simp)
-  verum  := .mkSigma “y param n | ∃ m, !pi₁Def m param ∧ !qqVerumDef y m” (by simp)
-  falsum := .mkSigma “y param n | ∃ m, !pi₁Def m param ∧ !qqFalsumDef y m” (by simp)
-  and    := .mkSigma “y param n p₁ p₂ y₁ y₂ | ∃ m, !pi₁Def m param ∧ !qqAndDef y m y₁ y₂” (by simp)
-  or     := .mkSigma “y param n p₁ p₂ y₁ y₂ | ∃ m, !pi₁Def m param ∧ !qqOrDef y m y₁ y₂” (by simp)
-  all    := .mkSigma “y param n p₁ y₁ | ∃ m, !pi₁Def m param ∧ !qqAllDef y m y₁” (by simp)
-  ex     := .mkSigma “y param n p₁ y₁ | ∃ m, !pi₁Def m param ∧ !qqExDef y m y₁” (by simp)
-  allChanges := .mkSigma “param' param n | ∃ m, !pi₁Def m param ∧ ∃ w, !pi₂Def w param ∧ ∃ qseq, !pL.qVecDef qseq n m w ∧ !pairDef param' (m + 1) qseq” (by simp)
-  exChanges := .mkSigma “param' param n | ∃ m, !pi₁Def m param ∧ ∃ w, !pi₂Def w param ∧ ∃ qseq, !pL.qVecDef qseq n m w ∧ !pairDef param' (m + 1) qseq” (by simp)
+  rel    := .mkSigma “y param k R v | ∃ v', !pL.termSubstVecDef v' k param v ∧ !qqRelDef y k R v'” (by simp)
+  nrel   := .mkSigma “y param k R v | ∃ v', !pL.termSubstVecDef v' k param v ∧ !qqNRelDef y k R v'” (by simp)
+  verum  := .mkSigma “y param | !qqVerumDef y” (by simp)
+  falsum := .mkSigma “y param | !qqFalsumDef y” (by simp)
+  and    := .mkSigma “y param p₁ p₂ y₁ y₂ | !qqAndDef y y₁ y₂” (by simp)
+  or     := .mkSigma “y param p₁ p₂ y₁ y₂ | !qqOrDef y y₁ y₂” (by simp)
+  all    := .mkSigma “y param p₁ y₁ | !qqAllDef y y₁” (by simp)
+  ex     := .mkSigma “y param p₁ y₁ | !qqExDef y y₁” (by simp)
+  allChanges := .mkSigma “param' param | !pL.qVecDef param' param” (by simp)
+  exChanges  := .mkSigma “param' param | !pL.qVecDef param' param” (by simp)
 
 variable (L)
 
 def construction : Language.UformulaRec1.Construction V L (blueprint pL) where
-  rel (param) := fun n k R v ↦ ^rel (π₁ param) k R (L.termSubstVec k n (π₁ param) (π₂ param) v)
-  nrel (param) := fun n k R v ↦ ^nrel (π₁ param) k R (L.termSubstVec k n (π₁ param) (π₂ param) v)
-  verum (param) := fun _ ↦ ^⊤[π₁ param]
-  falsum (param) := fun _ ↦ ^⊥[π₁ param]
-  and (param) := fun _ _ _ y₁ y₂ ↦ y₁ ^⋏[π₁ param] y₂
-  or (param) := fun _ _ _ y₁ y₂ ↦ y₁ ^⋎[π₁ param] y₂
-  all (param) := fun _ _ y₁ ↦ ^∀[π₁ param] y₁
-  ex (param) := fun _ _ y₁ ↦ ^∃[π₁ param] y₁
-  allChanges (param n) := ⟪π₁ param + 1, L.qVec n (π₁ param) (π₂ param)⟫
-  exChanges (param n) := ⟪π₁ param + 1, L.qVec n (π₁ param) (π₂ param)⟫
-  rel_defined := by intro v; simp [blueprint, (termSubstVec_defined L).df.iff]; rfl
-  nrel_defined := by intro v; simp [blueprint, (termSubstVec_defined L).df.iff]; rfl
+  rel (param)  := fun k R v ↦ ^rel k R (L.termSubstVec k param v)
+  nrel (param) := fun k R v ↦ ^nrel k R (L.termSubstVec k param v)
+  verum _      := ^⊤
+  falsum _     := ^⊥
+  and _        := fun _ _ y₁ y₂ ↦ y₁ ^⋏ y₂
+  or _         := fun _ _ y₁ y₂ ↦ y₁ ^⋎ y₂
+  all _        := fun _ y₁ ↦ ^∀ y₁
+  ex _         := fun _ y₁ ↦ ^∃ y₁
+  allChanges (param) := L.qVec param
+  exChanges (param) := L.qVec param
+  rel_defined := by intro v; simp [blueprint, L.termSubstVec_defined.df.iff]; rfl
+  nrel_defined := by intro v; simp [blueprint, L.termSubstVec_defined.df.iff]; rfl
   verum_defined := by intro v; simp [blueprint]
   falsum_defined := by intro v; simp [blueprint]
   and_defined := by intro v; simp [blueprint]; rfl
   or_defined := by intro v; simp [blueprint]; rfl
   all_defined := by intro v; simp [blueprint]; rfl
   ex_defined := by intro v; simp [blueprint]; rfl
-  allChanges_defined := by intro v; simp [blueprint, (qVec_defined L).df.iff]
-  exChanges_defined := by intro v; simp [blueprint, (qVec_defined L).df.iff]
+  allChanges_defined := by intro v; simp [blueprint, L.qVec_defined.df.iff]
+  exChanges_defined := by intro v; simp [blueprint, L.qVec_defined.df.iff]
 
 end Substs
 
@@ -389,310 +390,324 @@ open Substs
 
 variable (L)
 
-def Language.substs (m w p : V) : V := (construction L).result ⟪m, w⟫ p
+def Language.substs (w p : V) : V := (construction L).result w p
 
 variable {L}
 
 section
 
-def _root_.LO.FirstOrder.Arith.LDef.substsDef (pL : LDef) : 𝚺₁.Semisentence 4 := .mkSigma
-  “q m w p | ∃ mw, !pairDef mw m w ∧ !(blueprint pL).result q mw p” (by simp)
+def _root_.LO.FirstOrder.Arith.LDef.substsDef (pL : LDef) : 𝚺₁.Semisentence 3 := (blueprint pL).result
 
 variable (L)
 
-lemma substs_defined : 𝚺₁-Function₃ L.substs via pL.substsDef := fun v ↦ by
-  simp [LDef.substsDef, (construction L).result_defined.df.iff]; rfl
+lemma Language.substs_defined : 𝚺₁-Function₂ L.substs via pL.substsDef := (construction L).result_defined
 
-@[simp] lemma eval_substsDef (v : Fin 4 → V) :
-    Semiformula.Evalbm (L := ℒₒᵣ) V v pL.substsDef ↔ v 0 = L.substs (v 1) (v 2) (v 3) := (substs_defined L).df.iff v
+instance Language.substs_definable : 𝚺₁-Function₂ L.substs := L.substs_defined.to_definable
 
-instance substs_definable : 𝚺₁-Function₃ L.substs :=
-  (substs_defined L).to_definable
-
-instance substs_definable' (Γ) : Γ-[m + 1]-Function₃ L.substs :=
-  .of_sigmaOne (substs_definable L) _ _
+instance Language.substs_definable' : Γ-[m + 1]-Function₂ L.substs := L.substs_definable.of_sigmaOne
 
 end
 
 variable {m w : V}
 
-@[simp] lemma substs_rel {n k R v} (hR : L.Rel k R) (hv : L.SemitermVec k n v) :
-    L.substs m w (^rel n k R v) = ^rel m k R (L.termSubstVec k n m w v) := by simp [Language.substs, hR, hv, construction]
+@[simp] lemma substs_rel {k R v} (hR : L.Rel k R) (hv : L.IsUTermVec k v) :
+    L.substs w (^relk R v) = ^rel k R (L.termSubstVec k w v) := by simp [Language.substs, hR, hv, construction]
 
-@[simp] lemma substs_nrel {n k R v} (hR : L.Rel k R) (hv : L.SemitermVec k n v) :
-    L.substs m w (^nrel n k R v) = ^nrel m k R (L.termSubstVec k n m w v) := by simp [Language.substs, hR, hv, construction]
+@[simp] lemma substs_nrel {k R v} (hR : L.Rel k R) (hv : L.IsUTermVec k v) :
+    L.substs w (^nrelk R v) = ^nrel k R (L.termSubstVec k w v) := by simp [Language.substs, hR, hv, construction]
 
-@[simp] lemma substs_verum (n) :
-    L.substs m w ^⊤[n] = ^⊤[m] := by simp [Language.substs, construction]
+@[simp] lemma substs_verum (w) : L.substs w ^⊤ = ^⊤ := by simp [Language.substs, construction]
 
-@[simp] lemma substs_falsum (n) :
-    L.substs m w ^⊥[n] = ^⊥[m] := by simp [Language.substs, construction]
+@[simp] lemma substs_falsum (w) : L.substs w ^⊥ = ^⊥ := by simp [Language.substs, construction]
 
-@[simp] lemma substs_and {n p q} (hp : L.Semiformula n p) (hq : L.Semiformula n q) :
-    L.substs m w (p ^⋏[n] q) = L.substs m w p ^⋏[m] L.substs m w q := by simp [Language.substs, hp, hq, construction]
+@[simp] lemma substs_and {p q} (hp : L.IsUFormula p) (hq : L.IsUFormula q) :
+    L.substs w (p ^⋏ q) = L.substs w p ^⋏ L.substs w q := by simp [Language.substs, hp, hq, construction]
 
-@[simp] lemma substs_or {n p q} (hp : L.Semiformula n p) (hq : L.Semiformula n q) :
-    L.substs m w (p ^⋎[n] q) = L.substs m w p ^⋎[m] L.substs m w q := by simp [Language.substs, hp, hq, construction]
+@[simp] lemma substs_or {p q} (hp : L.IsUFormula p) (hq : L.IsUFormula q) :
+    L.substs w (p ^⋎ q) = L.substs w p ^⋎ L.substs w q := by simp [Language.substs, hp, hq, construction]
 
-@[simp] lemma substs_all {n p} (hp : L.Semiformula (n + 1) p) :
-    L.substs m w (^∀[n] p) = ^∀[m] (L.substs (m + 1) (L.qVec n m w) p) := by simp [Language.substs, hp, construction]
+@[simp] lemma substs_all {p} (hp : L.IsUFormula p) :
+    L.substs w (^∀ p) = ^∀ (L.substs (L.qVec w) p) := by simp [Language.substs, hp, construction]
 
-@[simp] lemma substs_ex {n p} (hp : L.Semiformula (n + 1) p) :
-    L.substs m w (^∃[n] p) = ^∃[m] (L.substs (m + 1) (L.qVec n m w) p) := by simp [Language.substs, hp, construction]
+@[simp] lemma substs_ex {p} (hp : L.IsUFormula p) :
+    L.substs w (^∃ p) = ^∃ (L.substs (L.qVec w) p) := by simp [Language.substs, hp, construction]
 
-lemma uformula_subst_induction {P : V → V → V → V → Prop} (hP : 𝚺₁-Relation₄ P)
-    (hRel : ∀ n m w k R v, L.Rel k R → L.SemitermVec k n v → P m w (^rel n k R v) (^rel m k R (L.termSubstVec k n m w v)))
-    (hNRel : ∀ n m w k R v, L.Rel k R → L.SemitermVec k n v → P m w (^nrel n k R v) (^nrel m k R (L.termSubstVec k n m w v)))
-    (hverum : ∀ n m w, P m w (^⊤[n]) (^⊤[m]))
-    (hfalsum : ∀ n m w, P m w (^⊥[n]) (^⊥[m]))
-    (hand : ∀ n m w p q, L.Semiformula n p → L.Semiformula n q →
-      P m w p (L.substs m w p) → P m w q (L.substs m w q) → P m w (p ^⋏[n] q) (L.substs m w p ^⋏[m] L.substs m w q))
-    (hor : ∀ n m w p q, L.Semiformula n p → L.Semiformula n q →
-      P m w p (L.substs m w p) → P m w q (L.substs m w q) → P m w (p ^⋎[n] q) (L.substs m w p ^⋎[m] L.substs m w q))
-    (hall : ∀ n m w p, L.Semiformula (n + 1) p →
-      P (m + 1) (L.qVec n m w) p (L.substs (m + 1) (L.qVec n m w) p) →
-      P m w (^∀[n] p) (^∀[m] (L.substs (m + 1) (L.qVec n m w) p)))
-    (hex : ∀ n m w p, L.Semiformula (n + 1) p →
-      P (m + 1) (L.qVec n m w) p (L.substs (m + 1) (L.qVec n m w) p) →
-      P m w (^∃[n] p) (^∃[m] (L.substs (m + 1) (L.qVec n m w) p))) :
-    ∀ {p m w}, L.UFormula p → P m w p (L.substs m w p) := by
-  suffices ∀ param p, L.UFormula p → P (π₁ param) (π₂ param) p ((construction L).result param p) by
-    intro p m w hp; simpa using this ⟪m, w⟫ p hp
-  apply (construction L).uformula_result_induction (P := fun param p y ↦ P (π₁ param) (π₂ param) p y)
-  · apply HierarchySymbol.Boldface.comp₄
-      (HierarchySymbol.BoldfaceFunction.comp₁ (HierarchySymbol.BoldfaceFunction.var _))
-      (HierarchySymbol.BoldfaceFunction.comp₁ (HierarchySymbol.BoldfaceFunction.var _))
-      (HierarchySymbol.BoldfaceFunction.var _)
-      (HierarchySymbol.BoldfaceFunction.var _)
-  · intro param n k R v hkR hv; simpa using hRel n (π₁ param) (π₂ param) k R v hkR hv
-  · intro param n k R v hkR hv; simpa using hNRel n (π₁ param) (π₂ param) k R v hkR hv
-  · intro param n; simpa using hverum n (π₁ param) (π₂ param)
-  · intro param n; simpa using hfalsum n (π₁ param) (π₂ param)
-  · intro param n p q hp hq ihp ihq
-    simpa [Language.substs] using
-      hand n (π₁ param) (π₂ param) p q hp hq (by simpa [Language.substs] using ihp) (by simpa [Language.substs] using ihq)
-  · intro param n p q hp hq ihp ihq
-    simpa [Language.substs] using
-      hor n (π₁ param) (π₂ param) p q hp hq (by simpa [Language.substs] using ihp) (by simpa [Language.substs] using ihq)
-  · intro param n p hp ihp
-    simpa using hall n (π₁ param) (π₂ param) p hp (by simpa [construction] using ihp)
-  · intro param n p hp ihp
-    simpa using hex n (π₁ param) (π₂ param) p hp (by simpa [construction] using ihp)
-
-lemma semiformula_subst_induction {P : V → V → V → V → V → Prop} (hP : 𝚺₁-Relation₅ P)
-    (hRel : ∀ n m w k R v, L.Rel k R → L.SemitermVec k n v → P n m w (^rel n k R v) (^rel m k R (L.termSubstVec k n m w v)))
-    (hNRel : ∀ n m w k R v, L.Rel k R → L.SemitermVec k n v → P n m w (^nrel n k R v) (^nrel m k R (L.termSubstVec k n m w v)))
-    (hverum : ∀ n m w, P n m w (^⊤[n]) (^⊤[m]))
-    (hfalsum : ∀ n m w, P n m w (^⊥[n]) (^⊥[m]))
-    (hand : ∀ n m w p q, L.Semiformula n p → L.Semiformula n q →
-      P n m w p (L.substs m w p) → P n m w q (L.substs m w q) → P n m w (p ^⋏[n] q) (L.substs m w p ^⋏[m] L.substs m w q))
-    (hor : ∀ n m w p q, L.Semiformula n p → L.Semiformula n q →
-      P n m w p (L.substs m w p) → P n m w q (L.substs m w q) → P n m w (p ^⋎[n] q) (L.substs m w p ^⋎[m] L.substs m w q))
-    (hall : ∀ n m w p, L.Semiformula (n + 1) p →
-      P (n + 1) (m + 1) (L.qVec n m w) p (L.substs (m + 1) (L.qVec n m w) p) →
-      P n m w (^∀[n] p) (^∀[m] (L.substs (m + 1) (L.qVec n m w) p)))
-    (hex : ∀ n m w p, L.Semiformula (n + 1) p →
-      P (n + 1) (m + 1) (L.qVec n m w) p (L.substs (m + 1) (L.qVec n m w) p) →
-      P n m w (^∃[n] p) (^∃[m] (L.substs (m + 1) (L.qVec n m w) p))) :
-    ∀ {n p m w}, L.Semiformula n p → P n m w p (L.substs m w p) := by
-  suffices ∀ param n p, L.Semiformula n p → P n (π₁ param) (π₂ param) p ((construction L).result param p) by
-    intro n p m w hp; simpa using this ⟪m, w⟫ n p hp
-  apply (construction L).semiformula_result_induction (P := fun param n p y ↦ P n (π₁ param) (π₂ param) p y)
-  · apply HierarchySymbol.Boldface.comp₅
-      (HierarchySymbol.BoldfaceFunction.var _)
-      (HierarchySymbol.BoldfaceFunction.comp₁ (HierarchySymbol.BoldfaceFunction.var _))
-      (HierarchySymbol.BoldfaceFunction.comp₁ (HierarchySymbol.BoldfaceFunction.var _))
-      (HierarchySymbol.BoldfaceFunction.var _)
-      (HierarchySymbol.BoldfaceFunction.var _)
-  · intro param n k R v hkR hv; simpa using hRel n (π₁ param) (π₂ param) k R v hkR hv
-  · intro param n k R v hkR hv; simpa using hNRel n (π₁ param) (π₂ param) k R v hkR hv
-  · intro param n; simpa using hverum n (π₁ param) (π₂ param)
-  · intro param n; simpa using hfalsum n (π₁ param) (π₂ param)
-  · intro param n p q hp hq ihp ihq
-    simpa [Language.substs] using
-      hand n (π₁ param) (π₂ param) p q hp hq (by simpa [Language.substs] using ihp) (by simpa [Language.substs] using ihq)
-  · intro param n p q hp hq ihp ihq
-    simpa [Language.substs] using
-      hor n (π₁ param) (π₂ param) p q hp hq (by simpa [Language.substs] using ihp) (by simpa [Language.substs] using ihq)
-  · intro param n p hp ihp
-    simpa using hall n (π₁ param) (π₂ param) p hp (by simpa [construction] using ihp)
-  · intro param n p hp ihp
-    simpa using hex n (π₁ param) (π₂ param) p hp (by simpa [construction] using ihp)
-
-@[simp] lemma Language.Semiformula.substs {n p m w : V} :
-    L.Semiformula n p → L.SemitermVec n m w → L.Semiformula m (L.substs m w p) := by
-  apply semiformula_subst_induction (P := fun n m w _ y ↦ L.SemitermVec n m w → L.Semiformula m y)
+lemma isUFormula_subst_induction_sigma1 {P : V → V → V → Prop} (hP : 𝚺₁-Relation₃ P)
+    (hRel : ∀ w k R v, L.Rel k R → L.IsUTermVec k v → P w (^relk R v) (^rel k R (L.termSubstVec k w v)))
+    (hNRel : ∀ w k R v, L.Rel k R → L.IsUTermVec k v → P w (^nrelk R v) (^nrel k R (L.termSubstVec k w v)))
+    (hverum : ∀ w, P w ^⊤ ^⊤)
+    (hfalsum : ∀ w, P w ^⊥ ^⊥)
+    (hand : ∀ w p q, L.IsUFormula p → L.IsUFormula q →
+      P w p (L.substs w p) → P w q (L.substs w q) → P w (p ^⋏ q) (L.substs w p ^⋏ L.substs w q))
+    (hor : ∀ w p q, L.IsUFormula p → L.IsUFormula q →
+      P w p (L.substs w p) → P w q (L.substs w q) → P w (p ^⋎ q) (L.substs w p ^⋎ L.substs w q))
+    (hall : ∀ w p, L.IsUFormula p → P (L.qVec w) p (L.substs (L.qVec w) p) → P w (^∀ p) (^∀ (L.substs (L.qVec w) p)))
+    (hex : ∀ w p, L.IsUFormula p → P (L.qVec w) p (L.substs (L.qVec w) p) → P w (^∃ p) (^∃ (L.substs (L.qVec w) p))) :
+    ∀ {w p}, L.IsUFormula p → P w p (L.substs w p) := by
+  suffices ∀ param p, L.IsUFormula p → P param p ((construction L).result param p) by
+    intro w p hp; simpa using this w p hp
+  apply (construction L).uformula_result_induction (P := fun param p y ↦ P param p y)
   · definability
-  case hRel => intro n m w k R v hR hv hw; simp [hR, hv, hw]
-  case hNRel => intro n m w k R v hR hv hw; simp [hR, hv, hw]
-  case hverum => simp
-  case hfalsum => simp
-  case hand =>
-    intro n m w p q _ _ ihp ihq hw
-    simp [ihp hw, ihq hw]
-  case hor =>
-    intro n m w p q _ _ ihp ihq hw
-    simp [ihp hw, ihq hw]
-  case hall =>
-    intro n m w p _ ih hw
-    simpa using ih hw.qVec
-  case hex =>
-    intro n m w p _ ih hw
-    simpa using ih hw.qVec
+  · intro param k R v hkR hv; simpa using hRel param k R v hkR hv
+  · intro param k R v hkR hv; simpa using hNRel param k R v hkR hv
+  · intro param; simpa using hverum param
+  · intro param; simpa using hfalsum param
+  · intro param p q hp hq ihp ihq
+    simpa [Language.substs] using
+      hand param p q hp hq (by simpa [Language.substs] using ihp) (by simpa [Language.substs] using ihq)
+  · intro param p q hp hq ihp ihq
+    simpa [Language.substs] using
+      hor param p q hp hq (by simpa [Language.substs] using ihp) (by simpa [Language.substs] using ihq)
+  · intro param p hp ihp
+    simpa using hall param p hp (by simpa [construction] using ihp)
+  · intro param p hp ihp
+    simpa using hex param p hp (by simpa [construction] using ihp)
 
-lemma substs_not_uformula {m w x} (h : ¬L.UFormula x) :
-    L.substs m w x = 0 := (construction L).result_prop_not _ h
+lemma semiformula_subst_induction {P : V → V → V → V → Prop} (hP : 𝚺₁-Relation₄ P)
+    (hRel : ∀ n w k R v, L.Rel k R → L.IsSemitermVec k n v → P n w (^relk R v) (^rel k R (L.termSubstVec k w v)))
+    (hNRel : ∀ n w k R v, L.Rel k R → L.IsSemitermVec k n v → P n w (^nrelk R v) (^nrel k R (L.termSubstVec k w v)))
+    (hverum : ∀ n w, P n w ^⊤ ^⊤)
+    (hfalsum : ∀ n w, P n w ^⊥ ^⊥)
+    (hand : ∀ n w p q, L.IsSemiformula n p → L.IsSemiformula n q →
+      P n w p (L.substs w p) → P n w q (L.substs w q) → P n w (p ^⋏ q) (L.substs w p ^⋏ L.substs w q))
+    (hor : ∀ n w p q, L.IsSemiformula n p → L.IsSemiformula n q →
+      P n w p (L.substs w p) → P n w q (L.substs w q) → P n w (p ^⋎ q) (L.substs w p ^⋎ L.substs w q))
+    (hall : ∀ n w p, L.IsSemiformula (n + 1) p →
+      P (n + 1) (L.qVec w) p (L.substs (L.qVec w) p) → P n w (^∀ p) (^∀ (L.substs (L.qVec w) p)))
+    (hex : ∀ n w p, L.IsSemiformula (n + 1) p →
+      P (n + 1) (L.qVec w) p (L.substs (L.qVec w) p) → P n w (^∃ p) (^∃ (L.substs (L.qVec w) p))) :
+    ∀ {n p w}, L.IsSemiformula n p → P n w p (L.substs w p) := by
+  suffices ∀ param n p, L.IsSemiformula n p → P n param p ((construction L).result param p) by
+    intro n p w hp; simpa using this w n p hp
+  apply (construction L).semiformula_result_induction (P := fun param n p y ↦ P n param p y)
+  · definability
+  · intro n param k R v hkR hv; simpa using hRel n param k R v hkR hv
+  · intro n param k R v hkR hv; simpa using hNRel n param k R v hkR hv
+  · intro n param; simpa using hverum n param
+  · intro n param; simpa using hfalsum n param
+  · intro n param p q hp hq ihp ihq
+    simpa [Language.substs] using
+      hand n param p q hp hq (by simpa [Language.substs] using ihp) (by simpa [Language.substs] using ihq)
+  · intro n param p q hp hq ihp ihq
+    simpa [Language.substs] using
+      hor n param p q hp hq (by simpa [Language.substs] using ihp) (by simpa [Language.substs] using ihq)
+  · intro n param p hp ihp
+    simpa using hall n param p hp (by simpa [construction] using ihp)
+  · intro n param p hp ihp
+    simpa using hex n param p hp (by simpa [construction] using ihp)
 
-lemma substs_neg {p} (hp : L.Semiformula n p) :
-    L.SemitermVec n m w → L.substs m w (L.neg p) = L.neg (L.substs m w p) := by
+@[simp] lemma Language.IsSemiformula.substs {n p m w : V} :
+    L.IsSemiformula n p → L.IsSemitermVec n m w → L.IsSemiformula m (L.substs w p) := by
+  let fw : V → V → V → V → V := fun _ w _ _ ↦ Max.max w (L.qVec w)
+  have hfw : 𝚺₁-Function₄ fw := by simp [fw]; definability
+  let fn : V → V → V → V → V := fun _ _ n _ ↦ n + 1
+  have hfn : 𝚺₁-Function₄ fn := by simp [fn]; definability
+  let fm : V → V → V → V → V := fun _ _ _ m ↦ m + 1
+  have hfm : 𝚺₁-Function₄ fm := by simp [fm]; definability
+  apply order_ball_induction₃_sigma1 hfw hfn hfm ?_ ?_ p w n m
+  · definability
+  intro p w n m ih hp hw
+  rcases Language.IsSemiformula.case_iff.mp hp with
+    (⟨k, R, v, hR, hv, rfl⟩ | ⟨k, R, v, hR, hv, rfl⟩ | rfl | rfl | ⟨p₁, p₂, h₁, h₂, rfl⟩ | ⟨p₁, p₂, h₁, h₂, rfl⟩ | ⟨p₁, h₁, rfl⟩ | ⟨p₁, h₁, rfl⟩)
+  · simp [hR, hv.isUTerm, hw.termSubstVec hv]
+  · simp [hR, hv.isUTerm, hw.termSubstVec hv]
+  · simp
+  · simp
+  · have ih₁ : L.IsSemiformula m (L.substs w p₁) := ih p₁ (by simp) w (by simp [fw]) n (by simp [fn]) m (by simp [fm]) h₁ hw
+    have ih₂ : L.IsSemiformula m (L.substs w p₂) := ih p₂ (by simp) w (by simp [fw]) n (by simp [fn]) m (by simp [fm]) h₂ hw
+    simp [h₁.isUFormula, h₂.isUFormula, ih₁, ih₂]
+  · have ih₁ : L.IsSemiformula m (L.substs w p₁) := ih p₁ (by simp) w (by simp [fw]) n (by simp [fn]) m (by simp [fm]) h₁ hw
+    have ih₂ : L.IsSemiformula m (L.substs w p₂) := ih p₂ (by simp) w (by simp [fw]) n (by simp [fn]) m (by simp [fm]) h₂ hw
+    simp [h₁.isUFormula, h₂.isUFormula, ih₁, ih₂]
+  · simpa [h₁.isUFormula] using ih p₁ (by simp) (L.qVec w) (by simp [fw]) (n + 1) (by simp [fn]) (m + 1) (by simp [fm]) h₁ hw.qVec
+  · simpa [h₁.isUFormula] using ih p₁ (by simp) (L.qVec w) (by simp [fw]) (n + 1) (by simp [fn]) (m + 1) (by simp [fm]) h₁ hw.qVec
+
+lemma substs_not_uformula {w x} (h : ¬L.IsUFormula x) :
+    L.substs w x = 0 := (construction L).result_prop_not _ h
+
+#check Language.IsSemiformula.induction_pi1
+
+lemma substs_neg {p} (hp : L.IsSemiformula n p) :
+    L.IsSemitermVec n m w → L.substs w (L.neg p) = L.neg (L.substs w p) := by
   revert m w
-  apply Language.Semiformula.induction_pi1 ?_ ?_ ?_ ?_ ?_ ?_ ?_ ?_ ?_ _ _ hp
+  apply Language.IsSemiformula.induction_pi1 ?_ ?_ ?_ ?_ ?_ ?_ ?_ ?_ ?_ hp
   · definability
-  · intros; simp [*]
-  · intros; simp [*]
+  · intros n k R v hR hv m w hw
+    rw [neg_rel hR hv.isUTerm, substs_nrel hR hv.isUTerm, substs_rel hR hv.isUTerm, neg_rel hR (hw.termSubstVec hv).isUTerm]
+  · intros n k R v hR hv m w hw
+    rw [neg_nrel hR hv.isUTerm, substs_rel hR hv.isUTerm, substs_nrel hR hv.isUTerm, neg_nrel hR (hw.termSubstVec hv).isUTerm]
   · intros; simp [*]
   · intros; simp [*]
   · intro n p q hp hq ihp ihq m w hw
-    simp [hp, hq, hw, hp.substs, hq.substs, ihp hw, ihq hw]
+    rw [neg_and hp.isUFormula hq.isUFormula,
+      substs_or hp.neg.isUFormula hq.neg.isUFormula,
+      substs_and hp.isUFormula hq.isUFormula,
+      neg_and (hp.substs hw).isUFormula (hq.substs hw).isUFormula,
+      ihp hw, ihq hw]
   · intro n p q hp hq ihp ihq m w hw
-    simp [hp, hq, hw, hp.substs, hq.substs, ihp hw, ihq hw]
+    rw [neg_or hp.isUFormula hq.isUFormula,
+      substs_and hp.neg.isUFormula hq.neg.isUFormula,
+      substs_or hp.isUFormula hq.isUFormula,
+      neg_or (hp.substs hw).isUFormula (hq.substs hw).isUFormula,
+      ihp hw, ihq hw]
   · intro n p hp ih m w hw
-    simp [hp, hw, hp.substs hw.qVec, ih hw.qVec]
+    rw [neg_all hp.isUFormula, substs_ex hp.neg.isUFormula,
+      substs_all hp.isUFormula, neg_all (hp.substs hw.qVec).isUFormula, ih hw.qVec]
   · intro n p hp ih m w hw
-    simp [hp, hw, hp.substs hw.qVec, ih hw.qVec]
+    rw [neg_ex hp.isUFormula, substs_all hp.neg.isUFormula,
+      substs_ex hp.isUFormula, neg_ex (hp.substs hw.qVec).isUFormula, ih hw.qVec]
 
-lemma shift_substs {p} (hp : L.Semiformula n p) :
-    L.SemitermVec n m w → L.shift (L.substs m w p) = L.substs m (L.termShiftVec n m w) (L.shift p) := by
+lemma shift_substs {p} (hp : L.IsSemiformula n p) :
+    L.IsSemitermVec n m w → L.shift (L.substs w p) = L.substs (L.termShiftVec n w) (L.shift p) := by
   revert m w
-  apply Language.Semiformula.induction_pi1 ?_ ?_ ?_ ?_ ?_ ?_ ?_ ?_ ?_ _ _ hp
+  apply Language.IsSemiformula.induction_pi1 ?_ ?_ ?_ ?_ ?_ ?_ ?_ ?_ ?_ hp
   · definability
   · intro n k R v hR hv m w hw
-    simp only [substs_rel, Language.SemitermVec.termSubstVec, shift_rel,
-      Language.SemitermVec.termShiftVec, qqRel_inj, true_and, hR, hv, hw]
-    apply nth_ext' k (by simp [*]) (by simp [*])
+    rw [substs_rel hR hv.isUTerm,
+      shift_rel hR (hw.termSubstVec hv).isUTerm,
+      shift_rel hR hv.isUTerm,
+      substs_rel hR hv.termShiftVec.isUTerm]
+    simp only [qqRel_inj, true_and]
+    apply nth_ext' k
+      (by rw [len_termShiftVec (hw.termSubstVec hv).isUTerm])
+      (by rw [len_termSubstVec hv.termShiftVec.isUTerm])
     intro i hi
-    rw [nth_termShiftVec (hw.termSubstVec hv) hi,
-      nth_termSubstVec hv hi,
-      nth_termSubstVec hv.termShiftVec hi,
-      nth_termShiftVec hv hi,
-      termShift_termSubsts (hv.2 i hi) hw]
+    rw [nth_termShiftVec (hw.termSubstVec hv).isUTerm hi,
+      nth_termSubstVec hv.isUTerm hi,
+      nth_termSubstVec hv.termShiftVec.isUTerm hi,
+      nth_termShiftVec hv.isUTerm hi,
+      termShift_termSubsts (hv.nth hi) hw]
   · intro n k R v hR hv m w hw
-    simp only [substs_nrel, Language.SemitermVec.termSubstVec, shift_nrel,
-      Language.SemitermVec.termShiftVec, qqNRel_inj, true_and, hR, hv, hw]
-    apply nth_ext' k (by simp [*]) (by simp [*])
+    rw [substs_nrel hR hv.isUTerm,
+      shift_nrel hR (hw.termSubstVec hv).isUTerm,
+      shift_nrel hR hv.isUTerm,
+      substs_nrel hR hv.termShiftVec.isUTerm]
+    simp only [qqNRel_inj, true_and]
+    apply nth_ext' k
+      (by rw [len_termShiftVec (hw.termSubstVec hv).isUTerm])
+      (by rw [len_termSubstVec hv.termShiftVec.isUTerm])
     intro i hi
-    rw [nth_termShiftVec (hw.termSubstVec hv) hi,
-      nth_termSubstVec hv hi,
-      nth_termSubstVec hv.termShiftVec hi,
-      nth_termShiftVec hv hi,
-      termShift_termSubsts (hv.2 i hi) hw]
+    rw [nth_termShiftVec (hw.termSubstVec hv).isUTerm hi,
+      nth_termSubstVec hv.isUTerm hi,
+      nth_termSubstVec hv.termShiftVec.isUTerm hi,
+      nth_termShiftVec hv.isUTerm hi,
+      termShift_termSubsts (hv.nth hi) hw]
   · intro n w hw; simp
   · intro n w hw; simp
   · intro n p q hp hq ihp ihq m w hw
-    simp [*]
-    rw [shift_and (hp.substs hw) (hq.substs hw), ihp hw, ihq hw]
+    rw [substs_and hp.isUFormula hq.isUFormula,
+      shift_and (hp.substs hw).isUFormula (hq.substs hw).isUFormula,
+      shift_and hp.isUFormula hq.isUFormula,
+      substs_and hp.shift.isUFormula hq.shift.isUFormula,
+      ihp hw, ihq hw]
   · intro n p q hp hq ihp ihq m w hw
-    simp [*]
-    rw [shift_or (hp.substs hw) (hq.substs hw), ihp hw, ihq hw]
+    rw [substs_or hp.isUFormula hq.isUFormula,
+      shift_or (hp.substs hw).isUFormula (hq.substs hw).isUFormula,
+      shift_or hp.isUFormula hq.isUFormula,
+      substs_or hp.shift.isUFormula hq.shift.isUFormula,
+      ihp hw, ihq hw]
   · intro n p hp ih m w hw
-    simp only [substs_all, shift_all, Language.Semiformula.shift_iff, hp]
-    rw [shift_all (hp.substs hw.qVec), ih hw.qVec, termShift_qVec hw]
+    rw [substs_all hp.isUFormula,
+      shift_all (hp.substs hw.qVec).isUFormula,
+      shift_all hp.isUFormula,
+      substs_all hp.shift.isUFormula,
+      ih hw.qVec,
+      termShift_qVec hw]
   · intro n p hp ih m w hw
-    simp only [substs_ex, shift_ex, Language.Semiformula.shift_iff, hp]
-    rw [shift_ex (hp.substs hw.qVec), ih hw.qVec, termShift_qVec hw]
+    rw [substs_ex hp.isUFormula,
+      shift_ex (hp.substs hw.qVec).isUFormula,
+      shift_ex hp.isUFormula,
+      substs_ex hp.shift.isUFormula,
+      ih hw.qVec,
+      termShift_qVec hw]
 
-lemma substs_substs {p} (hp : L.Semiformula l p) :
-    L.SemitermVec n m w → L.SemitermVec l n v → L.substs m w (L.substs n v p) = L.substs m (L.termSubstVec l n m w v) p := by
+lemma substs_substs {p} (hp : L.IsSemiformula l p) :
+    L.IsSemitermVec n m w → L.IsSemitermVec l n v → L.substs w (L.substs v p) = L.substs (L.termSubstVec l w v) p := by
   revert m w n v
-  apply Language.Semiformula.induction_pi1 ?_ ?_ ?_ ?_ ?_ ?_ ?_ ?_ ?_ _ _ hp
-  · apply HierarchySymbol.Boldface.all
-    apply HierarchySymbol.Boldface.all
-    apply HierarchySymbol.Boldface.all
-    apply HierarchySymbol.Boldface.all
-    apply HierarchySymbol.Boldface.imp (by definability)
-    apply HierarchySymbol.Boldface.imp (by definability)
-    apply HierarchySymbol.Boldface.comp₂ (by simp; definability)
-    apply HierarchySymbol.BoldfaceFunction.comp₃ (by definability) ?_ (by definability)
-    apply HierarchySymbol.BoldfaceFunction₅.comp (termSubstVec_definable _) <;> definability
-  · intro l k R ts hR hts m w n v _ hv
-    simp only [substs_rel, Language.SemitermVec.termSubstVec, qqRel_inj, true_and, hR, hts, hv]
-    apply nth_ext' k (by simp [hv, hts]) (by simp [hts])
+  apply Language.IsSemiformula.induction_pi1 ?_ ?_ ?_ ?_ ?_ ?_ ?_ ?_ ?_ hp
+  · sorry
+  · intro l k R ts hR hts m w n v hw hv
+    rw [substs_rel hR hts.isUTerm,
+      substs_rel hR (hv.termSubstVec hts).isUTerm,
+      substs_rel hR hts.isUTerm]
+    simp only [qqRel_inj, true_and]
+    apply nth_ext' k (by rw [len_termSubstVec (hv.termSubstVec hts).isUTerm]) (by rw [len_termSubstVec hts.isUTerm])
     intro i hi
-    rw [nth_termSubstVec (hv.termSubstVec hts) hi,
-      nth_termSubstVec hts hi,
-      nth_termSubstVec hts hi,
-      termSubst_termSubst hv (hts.2 i hi)]
-  · intro l k R ts hR hts m w n v _ hv
-    simp only [substs_nrel, Language.SemitermVec.termSubstVec, qqNRel_inj, true_and, hR, hts, hv]
-    apply nth_ext' k (by simp [hv, hts]) (by simp [hts])
+    rw [nth_termSubstVec (hv.termSubstVec hts).isUTerm hi,
+      nth_termSubstVec hts.isUTerm hi,
+      nth_termSubstVec hts.isUTerm hi,
+      termSubst_termSubst hv (hts.nth hi)]
+  · intro l k R ts hR hts m w n v hw hv
+    rw [substs_nrel hR hts.isUTerm,
+      substs_nrel hR (hv.termSubstVec hts).isUTerm,
+      substs_nrel hR hts.isUTerm]
+    simp only [qqNRel_inj, true_and]
+    apply nth_ext' k (by rw [len_termSubstVec (hv.termSubstVec hts).isUTerm]) (by rw [len_termSubstVec hts.isUTerm])
     intro i hi
-    rw [nth_termSubstVec (hv.termSubstVec hts) hi,
-      nth_termSubstVec hts hi,
-      nth_termSubstVec hts hi,
-      termSubst_termSubst hv (hts.2 i hi)]
-  · intro l m w n v _ _; simp [*]
-  · intro l m w n v _ _; simp [*]
+    rw [nth_termSubstVec (hv.termSubstVec hts).isUTerm hi,
+      nth_termSubstVec hts.isUTerm hi,
+      nth_termSubstVec hts.isUTerm hi,
+      termSubst_termSubst hv (hts.nth hi)]
+  · intros; simp
+  · intros; simp
   · intro l p q hp hq ihp ihq m w n v hw hv
-    simp only [substs_and, hp, hq]
-    rw [substs_and (hp.substs hv) (hq.substs hv), ihp hw hv, ihq hw hv]
+    rw [substs_and hp.isUFormula hq.isUFormula,
+      substs_and (hp.substs hv).isUFormula (hq.substs hv).isUFormula,
+      substs_and hp.isUFormula hq.isUFormula,
+      ihp hw hv, ihq hw hv]
   · intro l p q hp hq ihp ihq m w n v hw hv
-    simp only [substs_or, hp, hq]
-    rw [substs_or (hp.substs hv) (hq.substs hv), ihp hw hv, ihq hw hv]
-  · intro l p hp ih m w n v hw hv
-    simp only [substs_all, hp]
-    rw [substs_all (hp.substs hv.qVec), ih hw.qVec hv.qVec, termSubstVec_qVec_qVec hv hw]
-  · intro l p hp ih m w n v hw hv
-    simp only [substs_ex, hp]
-    rw [substs_ex (hp.substs hv.qVec), ih hw.qVec hv.qVec, termSubstVec_qVec_qVec hv hw]
+    rw [substs_or hp.isUFormula hq.isUFormula,
+      substs_or (hp.substs hv).isUFormula (hq.substs hv).isUFormula,
+      substs_or hp.isUFormula hq.isUFormula,
+      ihp hw hv, ihq hw hv]
 
-lemma subst_eq_self {n w : V} (hp : L.Semiformula n p) (hw : L.SemitermVec n n w) (H : ∀ i < n, w.[i] = ^#i) :
-    L.substs n w p = p := by
+lemma subst_eq_self {n w : V} (hp : L.IsSemiformula n p) (hw : L.IsSemitermVec n n w) (H : ∀ i < n, w.[i] = ^#i) :
+    L.substs w p = p := by
   revert w
-  apply Language.Semiformula.induction_pi1 ?_ ?_ ?_ ?_ ?_ ?_ ?_ ?_ ?_ _ _ hp
+  apply Language.IsSemiformula.induction_pi1 ?_ ?_ ?_ ?_ ?_ ?_ ?_ ?_ ?_ hp
   · definability
   · intro n k R v hR hv w _ H
-    simp only [substs_rel, qqRel_inj, true_and, hR, hv]
-    apply nth_ext' k (by simp [*]) (by simp [hv.1])
+    simp only [substs_rel, qqRel_inj, true_and, hR, hv.isUTerm]
+    apply nth_ext' k (by simp [*, hv.isUTerm]) (by simp [hv.lh])
     intro i hi
-    rw [nth_termSubstVec hv hi, termSubst_eq_self (hv.2 i hi) H]
+    rw [nth_termSubstVec hv.isUTerm hi, termSubst_eq_self (hv.nth hi) H]
   · intro n k R v hR hv w _ H
-    simp only [substs_nrel, qqNRel_inj, true_and, hR, hv]
-    apply nth_ext' k (by simp [*]) (by simp [hv.1])
+    simp only [substs_nrel, qqNRel_inj, true_and, hR, hv.isUTerm]
+    apply nth_ext' k (by simp [*, hv.isUTerm]) (by simp [hv.lh])
     intro i hi
-    rw [nth_termSubstVec hv hi, termSubst_eq_self (hv.2 i hi) H]
+    rw [nth_termSubstVec hv.isUTerm hi, termSubst_eq_self (hv.nth hi) H]
   · intro n w _ _; simp
   · intro n w _ _; simp
   · intro n p q hp hq ihp ihq w hw H
-    simp [*, ihp hw H, ihq hw H]
+    simp [*, hp.isUFormula, hq.isUFormula, ihp hw H, ihq hw H]
   · intro n p q hp hq ihp ihq w hw H
-    simp [*, ihp hw H, ihq hw H]
+    simp [*, hp.isUFormula, hq.isUFormula, ihp hw H, ihq hw H]
   · intro n p hp ih w hw H
-    have H : ∀ i < n + 1, (L.qVec n n w).[i] = ^#i := by
+    have H : ∀ i < n + 1, (L.qVec w).[i] = ^#i := by
       intro i hi
       rcases zero_or_succ i with (rfl | ⟨i, rfl⟩)
       · simp [Language.qVec]
       · have hi : i < n := by simpa using hi
         simp only [Language.qVec, nth_cons_succ]
-        rw [nth_termBShiftVec hw hi]
-        simp [H i hi, hi]
-    simp [*, ih hw.qVec H]
+        rw [nth_termBShiftVec (by simpa [hw.lh] using hw.isUTerm) (by simp [hw.lh, hi])]
+        simp [hw.lh, H i hi, hi]
+    simp [*, hp.isUFormula, ih hw.qVec H]
   · intro n p hp ih w hw H
-    have H : ∀ i < n + 1, (L.qVec n n w).[i] = ^#i := by
+    have H : ∀ i < n + 1, (L.qVec w).[i] = ^#i := by
       intro i hi
       rcases zero_or_succ i with (rfl | ⟨i, rfl⟩)
       · simp [Language.qVec]
       · have hi : i < n := by simpa using hi
         simp only [Language.qVec, nth_cons_succ]
-        rw [nth_termBShiftVec hw hi]
+        rw [nth_termBShiftVec (by simpa [hw.lh] using hw.isUTerm) (by simp [hw.lh, hi])]
         simp [H i hi, hi]
-    simp [*, ih hw.qVec H]
+    simp [*, hp.isUFormula, ih hw.qVec H]
 
 end substs
 
-
 variable (L)
 
-def Language.substs₁ (t u : V) : V := L.substs 0 ?[t] u
+def Language.substs₁ (t u : V) : V := L.substs ?[t] u
 
 variable {L}
 
@@ -701,19 +716,21 @@ section substs₁
 section
 
 def _root_.LO.FirstOrder.Arith.LDef.substs₁Def (pL : LDef) : 𝚺₁.Semisentence 3 := .mkSigma
-  “ z t p | ∃ v, !consDef v t 0 ∧ !pL.substsDef z 0 v p” (by simp)
+  “ z t p | ∃ v, !consDef v t 0 ∧ !pL.substsDef z v p” (by simp)
 
 variable (L)
 
-lemma substs₁_defined : 𝚺₁-Function₂ L.substs₁ via pL.substs₁Def := by
-  intro v; simp [LDef.substs₁Def, (substs_defined L).df.iff]; rfl
+lemma Language.substs₁_defined : 𝚺₁-Function₂ L.substs₁ via pL.substs₁Def := by
+  intro v; simp [LDef.substs₁Def, L.substs_defined.df.iff]; rfl
 
-@[simp] instance substs₁_definable : 𝚺₁-Function₂ L.substs₁ := (substs₁_defined L).to_definable
+instance Language.substs₁_definable : 𝚺₁-Function₂ L.substs₁ := L.substs₁_defined.to_definable
+
+instance : Γ-[m + 1]-Function₂ L.substs₁ := L.substs₁_definable.of_sigmaOne
 
 end
 
-lemma Language.Semiformula.substs₁ (ht : L.Term t) (hp : L.Semiformula 1 p) : L.Semiformula 0 (L.substs₁ t p) :=
-  Language.Semiformula.substs hp (by simp [ht])
+lemma Language.IsSemiformula.substs₁ (ht : L.IsSemiterm n t) (hp : L.IsSemiformula 1 p) : L.IsSemiformula n (L.substs₁ t p) :=
+  Language.IsSemiformula.substs hp (by simp [ht])
 
 end substs₁
 
@@ -732,23 +749,26 @@ def _root_.LO.FirstOrder.Arith.LDef.freeDef (pL : LDef) : 𝚺₁.Semisentence 2
 
 variable (L)
 
-lemma free_defined : 𝚺₁-Function₁ L.free via pL.freeDef := by
-  intro v; simp [LDef.freeDef, (shift_defined L).df.iff, (substs₁_defined L).df.iff, Language.free]
+lemma Language.free_defined : 𝚺₁-Function₁ L.free via pL.freeDef := by
+  intro v; simp [LDef.freeDef, L.shift_defined.df.iff, L.substs₁_defined.df.iff, Language.free]
 
-instance free_definable : 𝚺-[0 + 1]-Function₁ L.free := (free_defined L).to_definable
+instance Language.free_definable : 𝚺₁-Function₁ L.free := L.free_defined.to_definable
+
+instance Language.free_definable' : Γ-[m + 1]-Function₁ L.free := L.free_definable.of_sigmaOne
 
 end
 
-@[simp] lemma Language.Semiformula.free (hp : L.Semiformula 1 p) : L.Formula (L.free p) :=
-  Language.Semiformula.substs₁ (by simp) (by simp [hp])
+@[simp] lemma Language.IsSemiformula.free (hp : L.IsSemiformula 1 p) : L.IsFormula (L.free p) :=
+  Language.IsSemiformula.substs₁ (by simp) hp.shift
 
 end free
 
+/-
 section fvfree
 
 variable (L)
 
-def Language.IsFVFree (n p : V) : Prop := L.Semiformula n p ∧ L.shift p = p
+def Language.IsFVFree (n p : V) : Prop := L.IsSemiformula n p ∧ L.shift p = p
 
 section
 
@@ -782,79 +802,72 @@ lemma Language.IsFVFree.ex {n p : V} (hp : L.IsFVFree (n + 1) p) :
 @[simp] lemma Language.IsFVFree.neg_iff : L.IsFVFree n (L.neg p) ↔ L.IsFVFree n p := by
   constructor
   · intro h
-    have hp : L.Semiformula n p := Language.Semiformula.neg_iff.mp h.1
+    have hp : L.Semiformula n p := Language.IsSemiformula.neg_iff.mp h.1
     have : L.shift (L.neg p) = L.neg p := h.2
     simp [shift_neg hp, neg_inj_iff hp.shift hp] at this
     exact ⟨hp, this⟩
   · intro h; exact ⟨by simp [h.1], by rw [shift_neg h.1, h.2]⟩
 
 end fvfree
+-/
 
 namespace Formalized
 
-def qqEQ (n x y : V) : V := ^rel n 2 (eqIndex : V) ?[x, y]
+def qqEQ (x y : V) : V := ^rel 2 (eqIndex : V) ?[x, y]
 
-def qqNEQ (n x y : V) : V := ^nrel n 2 (eqIndex : V) ?[x, y]
+def qqNEQ (x y : V) : V := ^nrel 2 (eqIndex : V) ?[x, y]
 
-def qqLT (n x y : V) : V := ^rel n 2 (ltIndex : V) ?[x, y]
+def qqLT (x y : V) : V := ^rel 2 (ltIndex : V) ?[x, y]
 
-def qqNLT (n x y : V) : V := ^nrel n 2 (ltIndex : V) ?[x, y]
+def qqNLT (x y : V) : V := ^nrel 2 (ltIndex : V) ?[x, y]
 
-notation:75 x:75 " ^=[" n "] " y:76 => qqEQ n x y
+notation:75 x:75 " ^= " y:76 => qqEQ x y
 
-notation:75 x:75 " ^= " y:76 => qqEQ 0 x y
+notation:75 x:75 " ^≠ " y:76 => qqNEQ x y
 
-notation:75 x:75 " ^≠[" n "] " y:76 => qqNEQ n x y
+notation:78 x:78 " ^< " y:79 => qqLT x y
 
-notation:75 x:75 " ^≠ " y:76 => qqNEQ 0 x y
+notation:78 x:78 " ^≮ " y:79 => qqNLT x y
 
-notation:78 x:78 " ^<[" n "] " y:79 => qqLT n x y
+def _root_.LO.FirstOrder.Arith.qqEQDef : 𝚺₁.Semisentence 3 :=
+  .mkSigma “p x y | ∃ v, !mkVec₂Def v x y ∧ !qqRelDef p 2 ↑eqIndex v” (by simp)
 
-notation:78 x:78 " ^< " y:79 => qqLT 0 x y
+def _root_.LO.FirstOrder.Arith.qqNEQDef : 𝚺₁.Semisentence 3 :=
+  .mkSigma “p x y | ∃ v, !mkVec₂Def v x y ∧ !qqNRelDef p 2 ↑eqIndex v” (by simp)
 
-notation:78 x:78 " ^≮[" n "] " y:79 => qqNLT n x y
+def _root_.LO.FirstOrder.Arith.qqLTDef : 𝚺₁.Semisentence 3 :=
+  .mkSigma “p x y | ∃ v, !mkVec₂Def v x y ∧ !qqRelDef p 2 ↑ltIndex v” (by simp)
 
-notation:78 x:78 " ^≮ " y:79 => qqNLT 0 x y
+def _root_.LO.FirstOrder.Arith.qqNLTDef : 𝚺₁.Semisentence 3 :=
+  .mkSigma “p x y | ∃ v, !mkVec₂Def v x y ∧ !qqNRelDef p 2 ↑ltIndex v” (by simp)
 
-def _root_.LO.FirstOrder.Arith.qqEQDef : 𝚺₁.Semisentence 4 :=
-  .mkSigma “p n x y | ∃ v, !mkVec₂Def v x y ∧ !qqRelDef p n 2 (!(.Operator.numeral ℒₒᵣ eqIndex)) v” (by simp)
-
-def _root_.LO.FirstOrder.Arith.qqNEQDef : 𝚺₁.Semisentence 4 :=
-  .mkSigma “p n x y | ∃ v, !mkVec₂Def v x y ∧ !qqNRelDef p n 2 (!(.Operator.numeral ℒₒᵣ eqIndex)) v” (by simp)
-
-def _root_.LO.FirstOrder.Arith.qqLTDef : 𝚺₁.Semisentence 4 :=
-  .mkSigma “p n x y | ∃ v, !mkVec₂Def v x y ∧ !qqRelDef p n 2 (!(.Operator.numeral ℒₒᵣ ltIndex)) v” (by simp)
-
-def _root_.LO.FirstOrder.Arith.qqNLTDef : 𝚺₁.Semisentence 4 :=
-  .mkSigma “p n x y | ∃ v, !mkVec₂Def v x y ∧ !qqNRelDef p n 2 (!(.Operator.numeral ℒₒᵣ ltIndex)) v” (by simp)
-
-lemma qqEQ_defined : 𝚺₁-Function₃ (qqEQ : V → V → V → V) via qqEQDef := by
+lemma qqEQ_defined : 𝚺₁-Function₂ (qqEQ : V → V → V) via qqEQDef := by
   intro v; simp [qqEQDef, numeral_eq_natCast, qqEQ]
 
-lemma qqNEQ_defined : 𝚺-[0 + 1]-Function₃ (qqNEQ : V → V → V → V) via qqNEQDef := by
+lemma qqNEQ_defined : 𝚺₁-Function₂ (qqNEQ : V → V → V) via qqNEQDef := by
   intro v; simp [qqNEQDef, numeral_eq_natCast, qqNEQ]
 
-lemma qqLT_defined : 𝚺-[0 + 1]-Function₃ (qqLT : V → V → V → V) via qqLTDef := by
+lemma qqLT_defined : 𝚺₁-Function₂ (qqLT : V → V → V) via qqLTDef := by
   intro v; simp [qqLTDef, numeral_eq_natCast, qqLT]
 
-lemma qqNLT_defined : 𝚺-[0 + 1]-Function₃ (qqNLT : V → V → V → V) via qqNLTDef := by
+lemma qqNLT_defined : 𝚺₁-Function₂ (qqNLT : V → V → V) via qqNLTDef := by
   intro v; simp [qqNLTDef, numeral_eq_natCast, qqNLT]
 
-instance (Γ m) : Γ-[m + 1]-Function₃ (qqEQ : V → V → V → V) := .of_sigmaOne qqEQ_defined.to_definable _ _
+instance (Γ m) : Γ-[m + 1]-Function₂ (qqEQ : V → V → V) := .of_sigmaOne qqEQ_defined.to_definable
 
-instance (Γ m) : Γ-[m + 1]-Function₃ (qqNEQ : V → V → V → V) := .of_sigmaOne qqNEQ_defined.to_definable _ _
+instance (Γ m) : Γ-[m + 1]-Function₂ (qqNEQ : V → V → V) := .of_sigmaOne qqNEQ_defined.to_definable
 
-instance (Γ m) : Γ-[m + 1]-Function₃ (qqLT : V → V → V → V) := .of_sigmaOne qqLT_defined.to_definable _ _
+instance (Γ m) : Γ-[m + 1]-Function₂ (qqLT : V → V → V) := .of_sigmaOne qqLT_defined.to_definable
 
-instance (Γ m) : Γ-[m + 1]-Function₃ (qqNLT : V → V → V → V) := .of_sigmaOne qqNLT_defined.to_definable _ _
+instance (Γ m) : Γ-[m + 1]-Function₂ (qqNLT : V → V → V) := .of_sigmaOne qqNLT_defined.to_definable
 
-@[simp] lemma eval_qqEQDef (v) : Semiformula.Evalbm V v qqEQDef.val ↔ v 0 = v 2 ^=[v 1] v 3 := qqEQ_defined.df.iff v
+@[simp] lemma eval_qqEQDef (v) : Semiformula.Evalbm V v qqEQDef.val ↔ v 0 = v 1 ^= v 2 := qqEQ_defined.df.iff v
 
-@[simp] lemma eval_qqNEQDef (v) : Semiformula.Evalbm V v qqNEQDef.val ↔ v 0 = v 2 ^≠[v 1] v 3 := qqNEQ_defined.df.iff v
+@[simp] lemma eval_qqNEQDef (v) : Semiformula.Evalbm V v qqNEQDef.val ↔ v 0 = v 1 ^≠ v 2 := qqNEQ_defined.df.iff v
 
-@[simp] lemma eval_qqLTDef (v) : Semiformula.Evalbm V v qqLTDef.val ↔ v 0 = v 2 ^<[v 1] v 3 := qqLT_defined.df.iff v
+@[simp] lemma eval_qqLTDef (v) : Semiformula.Evalbm V v qqLTDef.val ↔ v 0 = v 1 ^< v 2 := qqLT_defined.df.iff v
 
-@[simp] lemma eval_qqNLTDef (v) : Semiformula.Evalbm V v qqNLTDef.val ↔ v 0 = v 2 ^≮[v 1] v 3 := qqNLT_defined.df.iff v
+@[simp] lemma eval_qqNLTDef (v) : Semiformula.Evalbm V v qqNLTDef.val ↔ v 0 = v 1 ^≮ v 2 := qqNLT_defined.df.iff v
 
 end Formalized
 
